Von Neumann's zoo of coins

theories/examples/von_neumann_coin.v
@@ -1,6 +1,9 @@
+(* A zoo of variants of Von Neumann's construction of a fair coin from a biased coin. *)
+
 From stdpp Require Import namespaces.
 From self.prob_lang Require Import lang notation spec_ra proofmode primitive_laws.
 From self.logrel Require Import model rel_rules rel_tactics compatibility.
+From self.typing Require Import fundamental.
 From self.prelude Require Import base.
 Set Default Proof Using "Type*".
 
@@ -9,19 +12,32 @@ Section proofs.
 
   Definition coinN := nroot.@"coin".
 
-  (* t4 = { true ⟼ 1/4, false ⟼ 3/4 } *)
+  (* Biased coin toss: t4 = { true ⟼ 1/4, false ⟼ 3/4 } *)
   Definition t4 :=
     (λ:<>,
       let: "b0" := flip #() in
       let: "b1" := flip #() in
       if: "b1" then "b0" else #false)%V.
 
+  (* Von Neumann coin. *)
   Definition vnc (t : expr) :=
     (rec: "f" <> :=
       let: "x" := t #() in
       let: "y" := t #() in
       if: "x" = "y" then "f" #() else "x")%V.
 
+  (* A variant that diverges instead of recursing. Can be used in simple
+  situations to prove a left-refinement because our judgement allows discarding
+  mass on the left. *)
+  Definition vnc_div (t : expr) :=
+    (λ:<>,
+      let: "x" := t #() in
+      let: "y" := t #() in
+      if: "x" = "y" then (rec: "f" <> := "f" #()) #() else "x")%V.
+
+  (* We can't show this refinement since the lhs needs to couple a combination
+  of flips with a single flip on the rhs and since we may need to recurse an
+  unbounded number of times. *)
   Goal ⊢ REL (vnc t4) << (λ:<>, flip #()) : lrel_unit → lrel_bool.
   Proof.
     rewrite /vnc.
@@ -35,21 +51,171 @@ Section proofs.
     unfold t4. rel_pures_l.
   Abort.
 
-  (* t2 = { true ⟼ 1/2, false ⟼ 1/2 } *)
+  (* A simpler coin toss: t2 = { true ⟼ 1/2, false ⟼ 1/2 } *)
   Definition t2 := (λ:<>, flip #())%V.
 
+  (* Still can't prove the refinement since we don't know how to recurse. *)
   Goal ⊢ REL (vnc t2) << (λ:<>, flip #()) : lrel_unit → lrel_bool.
   Proof.
+    iLöb as "HH".
     rewrite /vnc.
     rel_pures_r. rel_pures_l.
+
     iApply refines_arrow_val.
     iIntros "!#" (??) "#[-> ->]".
+    rel_rec_l.
     rel_pures_r. rel_pures_l.
     set (vnc2 := vnc t2) ; unfold vnc in vnc2 ; fold vnc2.
     unfold t2. rel_pures_l.
+
+    rel_bind_l (flip _)%E.
+    rel_bind_r (flip _)%E.
+    rel_apply_l refines_couple_flips_lr.
+    iIntros (b).
+    rel_pures_l.
+    rel_bind_l (flip _)%E.
+    rel_apply_l refines_flipU_l.
+    iIntros (b').
+    rel_pures_l.
+    case_bool_decide ; rel_pures_l.
+    - admit.
+    - rel_values.
   Abort.
 
-  Goal ⊢ REL flip #() = flip #() << flip #() : lrel_bool.
+  (* We can prove the refinement in case we diverge instead. *)
+  Goal ⊢ REL (vnc_div t2) << (λ:<>, flip #()) : lrel_unit → lrel_bool.
+  Proof.
+    rewrite /vnc_div.
+    rel_pures_r. rel_pures_l.
+    iApply refines_arrow_val.
+    iIntros "!#" (??) "#[-> ->]".
+    rel_rec_l.
+    rel_pures_r. rel_pures_l.
+    set (vnc2 := vnc_div t2) ; unfold vnc_div in vnc2 ; fold vnc2.
+    unfold t2. rel_pures_l.
+    rel_bind_l (flip _)%E.
+    rel_bind_r (flip _)%E.
+    rel_apply_l refines_couple_flips_lr.
+    iIntros (b).
+    rel_pures_l.
+    rel_bind_l (flip _)%E.
+    rel_apply_l refines_flipU_l.
+    iIntros (b').
+    rel_pures_l.
+    case_bool_decide ; rel_pures_l.
+    - iLöb as "H".
+      rel_rec_l.
+      iExact "H".
+    - rel_values.
+  Qed.
+
+  (* But unfortunately we can't even apply the divergence trick to the t4
+  biased coin, since we would have to decide on coupling the rhs flip with a
+  single flip on the left, but there's no single good choice. *)
+  Goal ⊢ REL (vnc_div t4) << (λ:<>, flip #()) : lrel_unit → lrel_bool.
+  Proof.
+    rewrite /vnc_div.
+    rel_pures_r. rel_pures_l.
+
+    iApply refines_arrow_val.
+    iIntros "!#" (??) "#[-> ->]".
+    rel_rec_l.
+    rel_pures_r. rel_pures_l.
+    set (vnc4 := vnc_div t4) ; unfold vnc_div in vnc4 ; fold vnc4.
+    unfold t4. rel_pures_l.
+
+    rel_bind_l (flip _)%E.
+    rel_bind_r (flip _)%E.
+    rel_apply_l refines_couple_flips_lr.
+    iIntros (b).
+    rel_pures_l.
+    rel_bind_l (flip _)%E.
+    rel_apply_l refines_flipU_l.
+    iIntros (b').
+    rel_pures_l.
+    destruct b'.
+    - rel_pures_l.
+      rel_bind_l (flip _)%E.
+      rel_apply_l refines_flipU_l.
+      iIntros (b').
+      rel_pures_l.
+      rel_bind_l (flip _)%E.
+      rel_apply_l refines_flipU_l.
+      iIntros (b'').
+      rel_pures_l.
+      destruct b''.
+      + rel_pures_l.
+        case_bool_decide ; rel_pures_l.
+        * iLöb as "H".
+          rel_rec_l.
+          iExact "H".
+        * rel_values.
+      + rel_pures_l.
+        case_bool_decide ; rel_pures_l.
+        * iLöb as "H".
+          rel_rec_l.
+          iExact "H".
+        * rel_values.
+    - rel_pures_l.
+      rel_bind_l (flip _)%E.
+      rel_apply_l refines_flipU_l.
+      iIntros (b').
+      rel_pures_l.
+      rel_bind_l (flip _)%E.
+      rel_apply_l refines_flipU_l.
+      iIntros (b'').
+      rel_pures_l.
+      destruct b''.
+      + rel_pures_l.
+        case_bool_decide ; rel_pures_l.
+        * iLöb as "H".
+          rel_rec_l.
+          iExact "H".
+        * give_up.
+      + rel_pures_l.
+        iLöb as "H".
+        rel_rec_l.
+        iExact "H".
   Abort.
 
+  (* A similar problem: no single flip on the left behaves like the rhs. *)
+  Goal ⊢ REL (flip #()) = (flip #()) << flip #() : lrel_bool.
+  Proof.
+    rel_bind_l (flip _)%E.
+    rel_bind_r (flip _)%E.
+    rel_apply_l refines_couple_flips_lr.
+    iIntros (b).
+    rel_bind_l (flip _)%E.
+    rel_apply_l refines_flipU_l.
+    iIntros (b').
+    rel_pures_l.
+  Abort.
+
+  (* We can however show this refinement where the result on the left only
+  depends on the outcome of one flip. *)
+  Goal ⊢ REL (let: "b" := flip #() in if: "b" = (flip #()) then "b" else "b") << flip #() : lrel_bool.
+  Proof.
+    rel_bind_l (flip _)%E.
+    rel_bind_r (flip _)%E.
+    rel_apply_l refines_couple_flips_lr.
+    iIntros (b).
+    rel_pures_l.
+    rel_bind_l (flip _)%E.
+    rel_apply_l refines_flipU_l.
+    iIntros (b').
+    rel_pures_l.
+    case_bool_decide ; rel_pures_l.
+    all: rel_values.
+  Qed.
+
+  (* We can even flip separately in each branch. *)
   Goal ⊢ REL if: flip #() then flip #() else flip #() << flip #() : lrel_bool.
+    rel_bind_l (flip _)%E.
+    rel_apply_l refines_flipU_l ; iIntros (b').
+    destruct b' ; rel_pures_l.
+    all: replace lrel_bool with (interp.interp types.TBool []) by easy ;
+      rel_apply_l refines_typed ;
+      apply types.TFlipU ; repeat constructor.
+  Qed.
+
+End proofs.
